  \begin{equation}\begin{gathered}\begin{aligned}
    \bar{\vFunc}_{t}({m}_{t})  & = \util(\bar{\cRat}_{t})\mathbb{C}_{t}^{T}\label{eq:vFuncPF}
    \\  & = \util(\bar{c}_{t}) \MinMPC_{t}^{-1} % 20190820
    \\  & = \util((\aboveMin \mRat_{t}+\aboveMin \hEnd_{t})\MinMPC_{t}) \MinMPC_{t}^{-1} % 20190820
    \\  & = \util(\aboveMin \mRat_{t}+\aboveMin \hEnd_{t})\MinMPC_{t}^{1-\CRRA} \MinMPC_{t}^{-1} % 20190820
    \\  & = \util(\aboveMin \mRat_{t}+\aboveMin \hEnd_{t})\MinMPC_{t}^{-\CRRA}  % 20190820
  \end{aligned}\end{gathered}\end{equation}
  where the second line uses the fact demonstrated in \cite{BufferStockTheory} that $\mathbb{C}_{t}=\MPC^{-1}_{t}$. % 20190820

  This can be transformed as
  \begin{equation*}\begin{gathered}\begin{aligned}
    \bar{\vInv}_{t}  & \equiv  \left((1-\CRRA)\bar{\vFunc}_{t}\right)^{1/(1-\CRRA)}
    \\  & = \cRat_{t}(\mathbb{C}_{t}^{T})^{1/(1-\CRRA)}
    \\  & = (\aboveMin \mRat_{t}+\aboveMin \hEnd_{t})\MinMPC_{t}^{-\CRRA/(1-\CRRA)}   % 20190820
  \end{aligned}\end{gathered}\end{equation*}
